## Variation of Subject

"srcText": "Next we will prove that g(k)⁢(ξ)-b has just a unique zero. On the contrary, let ξ0 and ξ0* be two distinct solutions of g(k)⁢(ξ)-b, and choose δ(>0) small enough such that D⁢(ξ0,δ)∩ D⁢(ξ0*,δ)=∅ where D⁢(ξ0,δ)={ξ:|ξ-ξ0|<δ} and D⁢(ξ0*,δ)={ξ:|ξ-ξ0*|<δ}. From (3.1) and Hurwitz’s theorem, there are points ξj∈D⁢(ξ0,δ),ξj*∈D⁢(ξ0*,δ) such that for sufficiently large j\n\n\t\nfj(k)⁢(zj+ρj⁢ξj)-b=0\nfj(k)⁢(zj+ρj⁢ξj*)-b=0.\n\t\n\nBy the hypothesis that for each pair of functions f and g in ℱ,f(k)⁢(ξ) and g(k)⁢(ξ) share b in D, we know that for any positive integer m\n\n\t\nfm(k)⁢(zj+ρj⁢ξj)-b=0\nfm(k)⁢(zj+ρj⁢ξj*)-b=0.\n\t\n\nFix m, take j→∞, and in view of that zj+ρj⁢ξj→0,zj+ρj⁢ξj*→0, we have\n\n\t\nfm(k)⁢(0)-b=0.\n\t\n\nSince the zeros of fm(k)-b have no accumulation point, we have that zj+ρj⁢ξj=0 and zj+ ρj⁢ξj*=0 Hence\n\n\t\nξj=-zjρj,ξj*=-zjρj.\n\t\n\nThis contradicts with ξj∈D⁢(ξ0,δ),ξj*∈D⁢(ξ0*,δ) and D⁢(ξ0,δ)∩D⁢(ξ0*,δ)=∅ So g(k)⁢(ξ)-b has just a unique zero, w", 

"suspText": "Next we will prove that gn⁢g(k)-a has just a unique zero. To the contrary, let ξ0 and ξ0* be two distinct solutions of gn⁢g(k)-a, and choose δ(>0) small enough such that D⁢(ξ0,δ)∩ D⁢(ξ0*,δ)=∅, where D⁢(ξ0,δ)={ξ:|ξ-ξ0|<δ} and D⁢(ξ0*,δ)={ξ:|ξ-ξ0*|<δ}. From (3.1), by\n\nYan and Ychussie Advances in Difference Equations ( 2015) 2015:226 Page 6 of 8 Hurwitz’s theorem, there exist points ξj∈D⁢(ξ0,δ),ξj*∈D⁢(ξ0*,δ) such that for sufficiently large j,\n\n\t\nfjn⁢(zj+ρj⁢ξj)⁢(fj(k)⁢(zj+ρj⁢ξj))-a=0\n\t\n\nand\n\n\t\nfjn⁢(zj+ρj⁢ξj)⁢(fj(k)⁢(zj+ρj⁢ξj))-a=0.\n\t\n\nBy the hypothesis that for each pair of functions f and g in ℱ,fn⁢f(k) and gn⁢g(k) share a in D, we know for any positive integer m\n\n\t\nfmn⁢(zj+ρj⁢ξj)⁢(fm(k)⁢(zj+ρj⁢ξj))-a=0\n\t\n\nand\n\n\t\nfmn⁢(zj+ρj⁢ξj)⁢(fm(k)⁢(zj+ρj⁢ξj))-a=0.\n\t\n\nFix m, take j→∞ and note zj+ρj⁢ξj→0,zj+ρj⁢ξj*→0, then we have\n\n\t\nfmn⁢(0)⁢(fm(k)⁢(0))-a=0\n\t\n\nSince the zeros of fmn⁢(0)⁢(fm(k)⁢(0))-a have no accumulation point, we have zj+ρj⁢ξj=0 and zj+ρj⁢ξj*=0 Hence\n\n\t\nξj=-zjρj,ξj*=-zjρj.\n\t\n\nThis contradicts with ξj∈D⁢(ξ0,δ),ξj*∈D⁢(ξ0*,δ) and D⁢(ξ0,δ)∩D⁢(ξ0*,δ)=∅. So gn⁢g(k)-a has just a unique zero, which can be denoted by ξ0."